

Rule 1:

$$a^m \times a^n$$

$$= (a \times a \dots m \text{ times}) \times (a \times a \dots n \text{ times})$$

$$= a \times a \times \dots \times a \text{ (} \underline{m+n \text{ times)}} \quad \rightarrow \text{ write clearly!}$$

$$= a^{m+n}$$

$$a^m \times a^n$$

$$= \underbrace{(a \times a \times \dots)}_{\text{'m' times}} \times \underbrace{(a \times a \times \dots)}_{\text{'n' times}}$$

$$= (a \times a \times \dots)$$

(m+n) times

a^{m+n}

$$= a^{m+n}$$

Rule 2:

$$\frac{a^m}{a^n}$$

$$\begin{aligned} & \frac{\underbrace{a \times a \dots (m \text{ times})}}{a \times a \dots (n \text{ times})} \\ &= a \times a \dots (m-n \text{ times}) \\ &= a^{m-n} \end{aligned}$$

→ Do it clearly!
See class notes

Rule 3:

$$(a^m)^n$$

$$= (\underbrace{a \times a}_{(m \text{ times})}) \times (\underbrace{a \times a}_{(m \text{ times})}) \dots (\underbrace{a \times a}_{(m \text{ times})}) \text{ (n times)}$$

$$= \underbrace{a^m \times a^m}_{(n \text{ times})}$$

$$= a^{m \times n}$$

Rule 4.

$$a^0$$

$$a^0 = a^{m-m}$$

$$= \frac{a^m}{a^m}$$

$$= \frac{a^m}{a^m}$$

$$= a^{m-m}$$

$$=$$

$$1$$

(only if $a \neq 0$)

$$= 1$$

Rule 5:

$$a^{-n}$$

$$= a^{0-n}$$

$$= \frac{a^0}{a^n}$$

$$= \frac{1}{a^n}$$